finish assignment targets

src/Sound/VCGen/AssignmentTarget.dfy
@@ -1,316 +1,502 @@
-// module AssignmentTarget'' {
-  // import opened Defs
-  // import Omni
+module AssignmentTarget {
+  import opened Defs
+  import Omni
 
-  // export
-  //   provides Defs, Omni, Process, Correct
-  //   reveals PairToSet, EqsTo
+  export
+    provides Defs, Omni, Process, Correct
+    reveals PairToSet, EqsTo
   
-  // predicate ShiftedIn(s: set<Idx>, n: nat, i: Idx) {
-  //   i + n in s
-  // }
+  predicate ShiftedIn(s: set<Idx>, n: nat, i: Idx) {
+    i + n in s
+  }
+  
 
-  // newtype VarsJumps = map<Idx, nat> {
-  //   function Update(n: nat): VarsJumps {
-  //     map i: Idx | i in Keys :: if i == 0 then n else Pred(this[i])
-  //   }
+  newtype VarsJumps = map<nat, set<Idx>> {
 
-  //   function Merge(m1: VarsJumps): VarsJumps {
-  //     map i: Idx | i in Keys + m1.Keys :: 
-  //       if i in Keys then
-  //         if i in m1.Keys then
-  //           min(this[i], m1[i])
-  //         else this[i]
-  //       else m1[i]
-  //   }
+    ghost function Get(n: nat): iset<Idx> {
+      iset i: Idx | In(i, n)
+    }
 
-  //   function Substract(n: nat): VarsJumps {
-  //     if Keys == {} then map[] else
-  //     map i: Idx {:trigger Pred(this[i + n])} | 
-  //       && i <= Max(Keys) - n
-  //       && i + n in Keys :: Pred(this[i + n])
-  //   }
+    ghost predicate In(i: Idx, n: nat) 
+    {
+      n in Keys && i in this[n]
+    }      
 
-  //   ghost function ToEqs(st: State, j: nat, posts: Omni.Continuation): Omni.Continuation 
-  //   {
-  //     seq(|posts|, k requires k < |posts| => 
-  //       if k < j then 
-  //         iset{}
-  //       else 
-  //         (iset st' |
-  //           && st' in posts[k]
-  //           && |st'| == |st|
-  //           && forall i: Idx :: i < |st| && !(i in Keys && this[i] <= k) ==> st[i] == st'[i]))
-  //   }
-  // }
+    function Merge(m1: VarsJumps): VarsJumps {
+      map i: Idx | i in Keys + m1.Keys :: 
+        if i in Keys then
+          if i in m1.Keys then
+            this[i] + m1[i]
+          else this[i]
+        else m1[i]
+    }
 
-  // function Pred(n: nat): nat {
-  //   if n == 0 then 0 else n - 1
-  // }
+    function Remove0(): VarsJumps {
+      var s0 := if 0 in Keys then this[0] else {};
+      map i: Idx | i in Keys - {0} :: this[i] + s0
+    }
 
-  // function Process'(stmt: Stmt): (VarsJumps, nat) 
-  //   ensures forall v <- Process'(stmt).0.Keys :: v < stmt.Depth()
-  //   decreases stmt
-  // {
-  //   match stmt
-  //   case Seq(ss) => SeqProcess'(ss)
-  //   case Choice(s0, s1) => 
-  //     var (vs0, b0) := Process'(s0);
-  //     var (vs1, b1) := Process'(s1);
-  //     (vs0.Merge(vs1), min(b0, b1))
-  //   case NewScope(n, s) => 
-  //     var (vs, b) := Process'(s);
-  //     (vs.Substract(n), Pred(b))
-  //   case Escape(n) => (map[], n)
-  //   case Loop(inv, body) => Process'(body)
-  //   case Assign(x, _) => (map[x := 0], 0)
-  //   case _ => (map[], 0)
-  // }
+    opaque function SeqMerge(m: VarsJumps): VarsJumps {
+      var s0 := if 0 in Keys then this[0] else {};
+      map i: nat | i in (Keys - {0}) + m.Keys :: 
+        if i in Keys then
+          if i in m.Keys then
+            this[i] + s0 + m[i]
+          else this[i]
+        else m[i] + s0
+    }
 
-  // function SeqProcess'(ss: seq<Stmt>): (VarsJumps, nat) 
-  //   ensures forall v <- SeqProcess'(ss).0.Keys :: v < SeqDepth(ss)
-  //   decreases ss
-  // {
-  //   if ss == [] then (map[], 0) else
-  //     var (v0, b0) := Process'(ss[0]);
-  //     if b0 == 0 then
-  //       var (v1, b1) := SeqProcess'(ss[1..]);
-  //       (v0.Update(b1).Merge(v1), b1)
-  //     else
-  //       (v0, b0)
-  // }
+    lemma SeqMergeKeys(m: VarsJumps)
+      ensures SeqMerge(m).Keys == Keys - {0} + m.Keys
+    {
+      reveal SeqMerge(m);
+    }
 
-  // ghost function AllStatesN(n: nat): Omni.Continuation 
-  //   requires n > 0
-  // {
-  //   seq(n, i => AllStates)
-  // }
+    lemma SeqMergeGet1(m: VarsJumps, i: Idx, k: nat)
+      requires i in Get(0)
+      requires k in m.Keys
+      ensures i in SeqMerge(m).Get(k)
+    {
+      reveal SeqMerge(m);
+    }
 
-  // lemma Process'Correct(stmt: Stmt, st: State, m: VarsJumps, n: nat, posts: Omni.Continuation) 
-  //   requires Process'(stmt) == (m, n)
-  //   ensures forall v <- m.Keys :: v < stmt.Depth()
-  //   requires Omni.Sem(stmt, st, posts)
-  //   ensures Omni.Sem(stmt, st, m.ToEqs(st, n, posts))
-  // {
-  //   match stmt
-  //   case Choice(s0, s1) => 
-  //     var (m0, n0) := Process'(s0);
-  //     var (m1, n1) := Process'(s1);
-  //     Omni.SemCons(s0, st, m0.ToEqs(st, n0, posts), m0.Merge(m1).ToEqs(st, min(n0, n1), posts)) by {
-  //       assert m0.ToEqs(st, n0, posts).Leq(m0.Merge(m1).ToEqs(st, min(n0, n1), posts));
-  //       Process'Correct(s0, st, m0, n0, posts);
-  //     }
-  //     Omni.SemCons(s1, st, m1.ToEqs(st, n1, posts), m0.Merge(m1).ToEqs(st, min(n0, n1), posts)) by {
-  //       assert m1.ToEqs(st, n1, posts).Leq(m0.Merge(m1).ToEqs(st, min(n0, n1), posts));
-  //       Process'Correct(s1, st, m1, n1, posts);
-  //     }
-  //   case Loop(_, body) => 
-  //     var inv :| 
-  //       && st in inv
-  //       && Omni.PreservesInv(inv, body, posts);
-  //     var inv' := inv * m.ToEqs(st, 0, posts.UpdateHead(inv)).head;
-  //     assert st in inv';
-  //     forall st': State | st' in inv' ensures Omni.Sem(body, st', m.ToEqs(st, n, posts).UpdateHead(inv')) {
-  //       Omni.SemCons(body, st', m.ToEqs(st, n, posts.UpdateHead(inv')), m.ToEqs(st, n, posts).UpdateHead(inv')) by {
-  //         assert Omni.Sem(body, st', m.ToEqs(st', n, posts.UpdateHead(inv'))) by {
-  //           Omni.SemCons(body, st', m.ToEqs(st', n, posts.UpdateHead(inv)), m.ToEqs(st', n, posts.UpdateHead(inv'))) by {
-  //             Process'Correct(body, st', m, n, posts.UpdateHead(inv)) by {
-  //               assert Omni.PreservesInv(inv, body, posts);
-  //             }
-  //             assert m.ToEqs(st', n, posts.UpdateHead(inv)).Leq(m.ToEqs(st', n, posts.UpdateHead(inv')));
-  //           }
-  //         }
-  //         Omni.SemCons(body, st', m.ToEqs(st', n, posts.UpdateHead(inv')), m.ToEqs(st, n, posts.UpdateHead(inv')));
-  //       }
-  //     }
-  //   case NewScope(k, body) =>
-  //     forall vs: State | |vs| == k ensures Omni.Sem(body, st.Update(vs), m.ToEqs(st, n, posts).UpdateAndAdd(k)) {
-  //       var (m', n') := Process'(body);
-  //       Omni.SemCons(body, st.Update(vs), m'.ToEqs(st.Update(vs), n', posts.UpdateAndAdd(k)), m.ToEqs(st, n, posts).UpdateAndAdd(k)) by {
-  //         Process'Correct(body, st.Update(vs), m', n', posts.UpdateAndAdd(k));
-  //         assert m'.ToEqs(st.Update(vs), n', posts.UpdateAndAdd(k)).Leq(m'.Substract(k).ToEqs(st, Pred(n'), posts).UpdateAndAdd(k)) by {
-  //           forall i: Idx | i < |posts| + 1 
-  //             ensures m'.ToEqs(st.Update(vs), n', posts.UpdateAndAdd(k))[i] <=
-  //                   m'.Substract(k).ToEqs(st, Pred(n'), posts).UpdateAndAdd(k)[i]
-  //           {
-  //             if i >= n' {
-  //               forall st': State | 
-  //                 && st' in posts.UpdateAndAdd(k)[i]
-  //                 && |st'| == |st| + k
-  //                 && forall j: Idx :: j < |st| + k && !(j in m'.Keys && m'[j] <= i) ==> st.Update(vs)[j] == st'[j]
-  //                 ensures
-  //                   st' in m'.Substract(k).ToEqs(st, Pred(n'), posts).UpdateAndAdd(k)[i]
-  //               {
-  //                 if i == 0 {
-  //                   assert st'[k..] in m'.Substract(k).ToEqs(st, 0, posts).head by {
-  //                     assert st'[k..] in posts.head by {
-  //                       assert st' in posts.UpdateAndAdd(k)[0];
-  //                       assert posts.UpdateAndAdd(k)[0] == UpdateSet(k, posts.head);
-  //                     }
-  //                     forall j: Idx | j < |st| && !(j in m'.Substract(k).Keys && m'.Substract(k)[j] <= 0) 
-  //                       ensures st[j] == st'[j + k]
-  //                     {
-  //                       if j + k in m'.Keys && m'[j + k] <= 0 {
-  //                         MaxLemma(m'.Keys, j, k);
-  //                         assert j in m'.Substract(k).Keys && m'.Substract(k)[j] <= 0;
-  //                       }
-  //                       assert !(j + k in m'.Keys && m'[j + k] <= 0);
-  //                     }
-  //                   }
-  //                 } else {
-  //                   assert st'[k..] in m'.Substract(k).ToEqs(st, 0, posts)[i - 1] by {
-  //                     assert st'[k..] in posts[i - 1] by {
-  //                       assert st' in posts.UpdateAndAdd(k)[i];
-  //                       assert posts.UpdateAndAdd(k)[i] == UpdateSet(k, posts[i - 1]);
-  //                     }
-  //                     forall j: Idx | j < |st| && !(j in m'.Substract(k).Keys && m'.Substract(k)[j] <= i - 1) 
-  //                       ensures st[j] == st'[j + k]
-  //                     {
-  //                       if j + k in m'.Keys && m'[j + k] <= i {
-  //                         MaxLemma(m'.Keys, j, k);
-  //                         assert j in m'.Substract(k).Keys && m'.Substract(k)[j] <= i - 1;
-  //                       }
-  //                       assert !(j + k in m'.Keys && m'[j + k] <= i);
-  //                     }
-  //                   }
-  //                 }
-  //               }
-  //             }
-  //           }
-  //         }
-  //       }
-  //     }
-  //   case Seq(ss) => SeqProcess'Correct(ss, st, m, n, posts);
-  //   case _ =>
-  // }
+    lemma SeqMergeGet1'(m: VarsJumps, i: Idx, k: nat)
+      requires i in Get(k)
+      requires k in Keys
+      requires k != 0
+      ensures i in SeqMerge(m).Get(k)
+    {
+      reveal SeqMerge(m);
+    }
 
-  // lemma SeqProcess'Correct(ss: seq<Stmt>, st: State, m: VarsJumps, n: nat, posts: Omni.Continuation) 
-  //   requires SeqProcess'(ss) == (m, n)
-  //   ensures forall v <- m.Keys :: v < SeqDepth(ss)
-  //   requires Omni.SeqSem(ss, st, posts)
-  //   ensures Omni.SeqSem(ss, st, m.ToEqs(st, n, posts))
-  // {
-  //   if ss != [] {
-  //     Omni.SemNest(ss[0], ss[1..], st, m.ToEqs(st, n, posts)) by {
-  //       assert Omni.Sem(ss[0], st, m.ToEqs(st, n, posts).UpdateHead(Omni.SeqWP(ss[1..],  m.ToEqs(st, n, posts)))) by {
-  //         assert Omni.Sem(ss[0], st, posts.UpdateHead(Omni.SeqWP(ss[1..], posts)));
-  //         var (m', n') := Process'(ss[0]);
-  //         Process'Correct(ss[0], st, m', n', posts.UpdateHead(Omni.SeqWP(ss[1..], posts)));
-  //         assert Omni.Sem(ss[0], st, m'.ToEqs(st, n', posts.UpdateHead(Omni.SeqWP(ss[1..], posts))));
-  //         if n' != 0 {
-  //           Omni.SemCons(ss[0], st, m'.ToEqs(st, n', posts.UpdateHead(Omni.SeqWP(ss[1..], posts))), 
-  //             m.ToEqs(st, n, posts).UpdateHead(Omni.SeqWP(ss[1..], m.ToEqs(st, n, posts))));
-  //         } else {
-  //           var (m'', n'') := SeqProcess'(ss[1..]);
-  //           assert m == m'.Update(n'').Merge(m'');
-  //           assert n == n'';
-  //           // ???
-  //           // forall st' | Omni.SeqSem(ss[1..], st', posts) { SeqProcess'Correct(ss[1..], st', m'', n'', posts); }
-  //           Omni.SemCons(ss[0], st, m'.ToEqs(st, n', posts.UpdateHead(Omni.SeqWP(ss[1..], posts))), 
-  //             m.ToEqs(st, n, posts).UpdateHead(Omni.SeqWP(ss[1..], m.ToEqs(st, n, posts)))) by 
-  //           {
-  //             forall i: Idx | i < |posts| 
-  //               ensures m'.ToEqs(st, n', posts.UpdateHead(Omni.SeqWP(ss[1..], posts)))[i] <= 
-  //                     m.ToEqs(st, n, posts).UpdateHead(Omni.SeqWP(ss[1..], m.ToEqs(st, n, posts)))[i] 
-  //             {
-  //               if i >= n' {
-  //                 forall st': State | st' in m'.ToEqs(st, n', posts.UpdateHead(Omni.SeqWP(ss[1..], posts)))[i] 
-  //                   ensures st' in m.ToEqs(st, n, posts).UpdateHead(Omni.SeqWP(ss[1..], m.ToEqs(st, n, posts)))[i] 
-  //                 {
-  //                   if i == 0 {
-  //                     assert Omni.SeqSem(ss[1..], st', posts);
-  //                     SeqProcess'Correct(ss[1..], st', m'', n'', posts);
-  //                     Omni.SeqSemCons(ss[1..], st', m''.ToEqs(st', n'', posts), m.ToEqs(st, n, posts));
-  //                     assert Omni.SeqSem(ss[1..], st', m.ToEqs(st, n, posts));
-  //                   } else {
-  //                     assert |st'| == |st|;
-  //                     assert st' in posts[i];
-  //                     assert forall j: Idx :: j < |st| && !(j in m'.Keys && m'[j] <= i) ==> st[j] == st'[j];
-  //                     assert st' in m.ToEqs(st, n, posts)[i] by {
-  //                       assert n' == 0;
-  //                       assert n == n'';
-  //                       forall j: Idx | j < |st| && !(j in m.Keys && m[j] <= i) 
-  //                         ensures st[j] == st'[j]
-  //                       {
-  //                         assume false;
-  //                       }
-  //                     }
-  //                   }
-  //                 }
-  //               }
-  //             }
-  //           }
-  //         }
-  //       }
-  //     }
-  //   }
-  // }
+    lemma SeqMergeGet2(m: VarsJumps, i: Idx, k: nat)
+      requires i in m.Get(k)
+      requires k in m.Keys
+      ensures i in SeqMerge(m).Get(k)
+    {
+      reveal SeqMerge(m);
+      var k' :| k' <= k && k' in m.Keys && i in m[k'];
+    }
 
-  // function Process(stmt: Stmt): set<Idx> 
-  //   ensures forall v <- Process(stmt) :: v < stmt.Depth()
-  // {
-  //   var (vs, n) := Process'(stmt);
-  //   if n == 0 then set i | i in vs.Keys && vs[i] == 0 else {}
-  // } 
+    function SubstractSet(n: nat, s: set<Idx>): set<Idx> 
+      ensures forall i: Idx :: i + n in s ==> i in SubstractSet(n, s)
+    {
+      set i: Idx {:trigger i + n in s} | i <= Max'(s) - n && i + n in s 
+    }
+
+    lemma InSubstractSet(s: set<Idx>, n: nat, i: Idx) 
+      requires i + n in s 
+      ensures i in SubstractSet(n, s)
+    {
+
+    }
+
+    predicate SubstractPred(i: Idx) {
+      i + 1 in Keys
+    }
+
+    opaque function Substract(n: nat): VarsJumps 
+    {
+      var m: VarsJumps := map i: nat {: trigger} | 
+        && i <= Max'(Keys) + 1
+        && i + 1 in Keys :: SubstractSet(n, this[i + 1]);
+      if 0 in m.Keys && 0 in Keys then 
+        m[0 := m[0] + SubstractSet(n, this[0])]
+      else if 0 in Keys then 
+        m[0 := SubstractSet(n, this[0])]
+      else m
+    }
+    lemma SubstractPlusOne(n: nat, i: Idx)
+      requires i + 1 in Keys
+      ensures i in Substract(n).Keys
+    {
+      reveal Substract(n);
+    }
+    lemma SubstractZero(n: nat)
+      requires 0 in Keys
+      ensures 0 in Substract(n).Keys
+    {
+      reveal Substract(n);
+    }
+    lemma SubstractGetZero(n: nat, i: Idx)
+      requires i + n in Get(0)
+      requires 0 in Keys
+      ensures i in Substract(n).Get(0)
+    {
+      SubstractZero(n);
+      reveal Substract(n);
+    }
+
+    lemma SubstractGet(n: nat, i: Idx, k: nat)
+      requires i + n in Get(k)
+      requires k > 0
+      // requires i + 1 in Keys
+      ensures i in Substract(n).Get(k - 1) 
+    {
+      reveal Substract(n);
+    }
+    lemma SubstracOfPlusOne(n: nat, i: Idx)
+      requires i + 1 in Keys
+      // requires i != 0
+      requires i in Substract(n).Keys
+      ensures Substract(n)[i] >= SubstractSet(n, this[i + 1])
+    {
+      reveal Substract(n);
+    }
+
+    ghost function ToEqs(st: State, posts: Omni.Continuation): Omni.Continuation 
+    {
+      seq(|posts|, (k : nat) requires k < |posts| => 
+        if k !in Keys then iset{} else
+        iset st' |
+          && st' in posts[k]
+          && |st'| == |st|
+          && forall i: Idx :: i < |st| && !(i in Get(k)) ==> st[i] == st'[i]
+      )
+    }
+
+    ghost function ToEqsAll(st: State): iset<State>
+    {
+        iset st' |
+          && |st'| == |st|
+          && forall i: Idx :: i < |st| && !(i in Get(0)) ==> st[i] == st'[i]
+    }
+
+    lemma GetLemma(n: nat)
+      requires n in Keys
+      requires n != 0
+      ensures Get(n) <= Remove0().Get(n)
+    {
+      if 0 in Keys {
+        forall i: Idx | i in Get(n) ensures i in Remove0().Get(n) {
+          var k :| k <= n && k in Keys && i in this[k];
+          if k != 0 {
+            assert k in Remove0().Keys;
+            assert this[k] <= Remove0()[k];
+          } else {
+            assert n in Remove0().Keys;
+          }
+        }
+      } else {
+        forall i: Idx | i in Get(n) ensures i in Remove0().Get(n) {
+          var k :| k <= n && k in Keys && i in this[k];
+          assert Remove0().Keys == Keys;
+          assert k in Remove0().Keys;
+        }
+      }
+    }
+  }
+
+  function Pred(n: nat): nat {
+    if n == 0 then 0 else n - 1
+  }
+  
+  function Process'(stmt: Stmt): VarsJumps 
+    ensures forall v <- Process'(stmt).Values, s <- v :: s < stmt.Depth()
+    decreases stmt
+  {
+    match stmt
+    case Seq(ss) => SeqProcess'(ss)
+    case Choice(s0, s1) => 
+      var vs0 := Process'(s0);
+      var vs1 := Process'(s1);
+      vs0.Merge(vs1)
+    case NewScope(n, s) => 
+      var vs := Process'(s);
+      reveal vs.Substract(n);
+      vs.Substract(n)
+    case Escape(n) => map[n := {}]
+    /**
+      Loop
+        (x++) + (y++; exit 1)
+    We need to add all m[0] vars to other m[i] because 
+    loop modify 0 vars in first few operations and then
+    exit modify other vars
+    */
+    case Loop(inv, body) => Process'(body).Remove0()
+    case Assign(x, _) => map[0 := {x}]
+    case _ => map[0 := {}]
+  }
+
+  function SeqProcess'(ss: seq<Stmt>): VarsJumps 
+    ensures forall v <- SeqProcess'(ss).Values, s <- v :: s < SeqDepth(ss)
+    decreases ss
+  {
+    if ss == [] then map[0 := {}] else
+      var v0 := Process'(ss[0]);
+      if 0 in v0.Keys then
+        reveal v0.SeqMerge(SeqProcess'(ss[1..]));
+        v0.SeqMerge(SeqProcess'(ss[1..]))
+      else v0
+  }
 
 
+  // verification-time-limit 40
+  lemma Process'Correct(stmt: Stmt, st: State, m: VarsJumps, posts: Omni.Continuation) 
+    requires Process'(stmt) == m
+    ensures forall v <- m.Values, s <- v :: s < stmt.Depth()
+    requires Omni.Sem(stmt, st, posts)
+    ensures Omni.Sem(stmt, st, m.ToEqs(st, posts))
+  {
+    match stmt 
+    case Choice(s0, s1) =>
+      var m0 := Process'(s0);
+      var m1 := Process'(s1);
+      Omni.SemCons(s0, st, m0.ToEqs(st, posts), m0.Merge(m1).ToEqs(st, posts)) by {
+        Process'Correct(s0, st, m0, posts);
+      }
+      Omni.SemCons(s1, st, m1.ToEqs(st, posts), m0.Merge(m1).ToEqs(st, posts)) by {
+        Process'Correct(s1, st, m1, posts);
+      }
+    case Loop(_, body) =>
+      var inv :| 
+        && st in inv
+        && Omni.PreservesInv(inv, body, posts);
+      var m' := Process'(body);
+      var inv' := inv * m'.ToEqsAll(st);
+      assert st in inv';
+      forall st': State | st' in inv' ensures Omni.Sem(body, st', (m'.Remove0()).ToEqs(st, posts).UpdateHead(inv')) {
+        Omni.SemCons(body, st', m'.ToEqs(st', posts.UpdateHead(inv)), (m'.Remove0()).ToEqs(st, posts).UpdateHead(inv')) by {
+          assert m'.ToEqs(st', posts.UpdateHead(inv)).Leq((m'.Remove0()).ToEqs(st, posts).UpdateHead(inv')) by {
+            forall i: Idx | i < |posts| 
+              ensures m'.ToEqs(st', posts.UpdateHead(inv))[i] <= (m'.Remove0()).ToEqs(st, posts).UpdateHead(inv')[i]
+            {
+              forall st'': State | st'' in m'.ToEqs(st', posts.UpdateHead(inv))[i]
+                ensures st'' in (m'.Remove0()).ToEqs(st, posts).UpdateHead(inv')[i]
+              {
+                if i in m'.Keys  {
+                  if i == 0 {
+                    if 0 in m'.Keys {
+                      assert st'' in inv;
+                    }
+                  } else {
+                    assert forall j: Idx :: j < |st'| && !(j in m'.Get(i)) ==> st'[j] == st''[j];
+                    assert forall j: Idx :: j < |st| && !(j in m'.Get(0)) ==> st[j] == st'[j];
+                    forall j: Idx | j < |st| && !(j in (m'.Remove0()).Get(i))
+                      ensures st[j] == st''[j]
+                    {
+                      m'.GetLemma(i);
+                      assert m'.Get(0) <= m'.Remove0().Get(i);
+                    }
+                  }
+                }
+              }
+            }
+          }
+          Process'Correct(body, st', m', posts.UpdateHead(inv)) by {
+            assert Omni.PreservesInv(inv, body, posts);
+          }
+        }
+      }
+    case NewScope(n, s) => 
+      forall vs: State | |vs| == n ensures Omni.Sem(s, st.Update(vs), m.ToEqs(st, posts).UpdateAndAdd(n)) {
+        var m' := Process'(s);
+        Omni.SemCons(s, st.Update(vs), m'.ToEqs(st.Update(vs), posts.UpdateAndAdd(n)), m.ToEqs(st, posts).UpdateAndAdd(n)) by {
+          Process'Correct(s, st.Update(vs), m', posts.UpdateAndAdd(n));
+          forall i: Idx | i < |posts| + 1 
+            ensures m'.ToEqs(st.Update(vs), posts.UpdateAndAdd(n))[i] <=
+              m'.Substract(n).ToEqs(st, posts).UpdateAndAdd(n)[i]
+          {
+            forall st': State | st' in m'.ToEqs(st.Update(vs), posts.UpdateAndAdd(n))[i] 
+              ensures st' in m'.Substract(n).ToEqs(st, posts).UpdateAndAdd(n)[i]
+            {
+              assert |st'| == |st| + n by {
+                calc {
+                  |st'|;
+                  == 
+                  |st.Update(vs)|;
+                }
+              }
+              assert st' in posts.UpdateAndAdd(n)[i];
+              if i == 0 {
+                assert st'[n..] in m'.Substract(n).ToEqs(st, posts).head by {
+                  assert forall i: Idx :: i < |st| + n && !(i in m'.Get(0)) ==> st.Update(vs)[i] == st'[i];
+                  if 0 in m'.Keys {
+                    assert Pred(0) in m'.Keys;
+                    assert 0 in m'.Substract(n).Keys by { m'.SubstractZero(n); }
+                    assert st'[n..] in m'.Substract(n).ToEqs(st, posts).head by {
+                      forall i: Idx | i < |st| && !(i in m'.Substract(n).Get(0)) 
+                        ensures st[i] == st'[n..][i] {
+                        assert !(i + n in m'.Get(0)) by {
+                          if i + n in m'.Get(0) {
+                            m'.SubstractGetZero(n, i); 
+                          }
+                        }
+                      }
+                    }
+                  }
+                }
+              } else {
+                assert st'[n..] in m'.Substract(n).ToEqs(st, posts)[i - 1] by {
+                  if i in m'.Keys {
+                    assert |st| + n == |st'|;
+                    assert st'[n..] in posts[i - 1] by {
+                      calc {
+                        st'[n..] in posts[i - 1];
+                        { assert |st'| >= n; }
+                        st' in UpdateSet(n, posts[i - 1]);
+                        { assert ([posts.head] + posts).Update(n)[i] == UpdateSet(n, posts[i - 1]); }
+                        st' in posts.UpdateAndAdd(n)[i];
+                      }
+                    }
+                    assert forall j: Idx :: j < |st| + n && !(j in m'.Get(i)) ==> st.Update(vs)[j] == st'[j];
+                    assert i - 1 <= Max'(m'.Keys) + 1;
+                    assert (i - 1) in m'.Substract(n).Keys by {
+                      m'.SubstractPlusOne(n, i - 1);
+                    }
+                    forall j: Idx | j < |st| && !(j in m'.Substract(n).Get(i - 1)) 
+                      ensures st[j] == st'[j + n] {
+                      assert !(j + n in m'.Get(i)) by {
+                        if j + n in m'.Get(i) {
+                          m'.SubstractGet(n, j, i);
+                        }
+                      }
+                    }
+                  }
+                }
+              }
+            }
+          }
+        }
+      }
+    case Seq(ss) => SeqProcess'Correct(ss, st, m, posts);
+    case _ =>
+  }
 
-  // // function Process(stmt: Stmt): (set<Idx>, bool) 
-  // //   ensures forall v <- Process(stmt).0 :: v < stmt.Depth()
-  // //   decreases stmt
-  // // {
-  // //   match stmt
-  // //   case Seq(ss) => SeqProcess(ss)
-  // //   case Choice(s0, s1) => 
-  // //     var (vs0, b0) := Process(s0);
-  // //     var (vs1, b1) := Process(s1);
-  // //     (vs0 + vs1, b0 || b1)
-  // //   case NewScope(n, s) => 
-  // //     var (vs, b) := Process(s);
-  // //     (Substract(vs, n), b)
-  // //   case Escape(_) => ({}, false)
-  // //   case Loop(inv, body) => Process(body)
-  // //   case Assign(x, _) => ({x}, true)
-  // //   case _ => ({}, true)
-  // // }
+  lemma SeqProcess'Correct(ss: seq<Stmt>, st: State, m: VarsJumps, posts: Omni.Continuation) 
+    requires SeqProcess'(ss) == m
+    ensures forall v <- m.Values, s <- v :: s < SeqDepth(ss)
+    requires Omni.SeqSem(ss, st, posts)
+    ensures Omni.SeqSem(ss, st, m.ToEqs(st, posts))
+  {
+    if ss != [] {
+      Omni.SemNest(ss[0], ss[1..], st, m.ToEqs(st, posts)) by {
+        assert Omni.Sem(ss[0], st, m.ToEqs(st, posts).UpdateHead(Omni.SeqWP(ss[1..],  m.ToEqs(st, posts)))) by {
+          assert Omni.Sem(ss[0], st, posts.UpdateHead(Omni.SeqWP(ss[1..], posts)));
+          var m' := Process'(ss[0]);
+          var m'' := SeqProcess'(ss[1..]);
+          Process'Correct(ss[0], st, m', posts.UpdateHead(Omni.SeqWP(ss[1..], posts)));
+          assert Omni.Sem(ss[0], st, m'.ToEqs(st, posts.UpdateHead(Omni.SeqWP(ss[1..], posts))));
+          Omni.SemCons(ss[0], st, m'.ToEqs(st, posts.UpdateHead(Omni.SeqWP(ss[1..], posts))), 
+            m.ToEqs(st, posts).UpdateHead(Omni.SeqWP(ss[1..], m.ToEqs(st, posts)))) by {
+            assert m'.ToEqs(st, posts.UpdateHead(Omni.SeqWP(ss[1..], posts))).Leq(
+              m.ToEqs(st, posts).UpdateHead(Omni.SeqWP(ss[1..], m.ToEqs(st, posts)))) by {
+              if 0 in m'.Keys {
+                assert m == m'.SeqMerge(m'');
+                forall i: Idx | i < |posts| 
+                  ensures m'.ToEqs(st, posts.UpdateHead(Omni.SeqWP(ss[1..], posts)))[i] <=
+                        m.ToEqs(st, posts).UpdateHead(Omni.SeqWP(ss[1..], m.ToEqs(st, posts)))[i]
+                {
+                  forall st': State | st' in m'.ToEqs(st, posts.UpdateHead(Omni.SeqWP(ss[1..], posts)))[i] 
+                    ensures st' in m.ToEqs(st, posts).UpdateHead(Omni.SeqWP(ss[1..], m.ToEqs(st, posts)))[i]
+                  {
+                    if i == 0 {
+                      assert forall j: Idx :: j < |st| && !(j in m'.Get(0)) ==> st[j] == st'[j];
+                      assert Omni.SeqSem(ss[1..], st', posts);
+                      SeqProcess'Correct(ss[1..], st', m'', posts);
+                      Omni.SeqSemCons(ss[1..], st', m''.ToEqs(st', posts), m'.SeqMerge(m'').ToEqs(st, posts)) by {
+                        forall i: Idx | i < |posts| 
+                          ensures m''.ToEqs(st', posts)[i] <= m'.SeqMerge(m'').ToEqs(st, posts)[i]
+                        {
+                          forall st'': State | st'' in m''.ToEqs(st', posts)[i]
+                            ensures st'' in m'.SeqMerge(m'').ToEqs(st, posts)[i] {
+                            if i in m''.Keys {
+                              assert i in m'.SeqMerge(m'').Keys by {
+                                m'.SeqMergeKeys(m'');
+                              }
+                              forall j: Idx | j < |st| && !(j in m'.SeqMerge(m'').Get(i))
+                                ensures st[j] == st''[j]
+                              {
+                                assert |st| == |st'| == |st''|;
+                                assert j !in m''.Get(i) by {
+                                  if j in m''.Get(i) {
+                                    m'.SeqMergeGet2(m'', j, i);
+                                  }
+                                }
+                                assert st'[j] == st''[j];
+                                assert j !in m'.Get(0) by {
+                                  if j in m'.Get(0) {
+                                    m'.SeqMergeGet1(m'', j, i);
+                                  }
+                                }
+                                assert st[j] == st'[j];
+                              }
+                            } 
+                          }
+                        }
+                      }
+                      assert Omni.SeqSem(ss[1..], st', m.ToEqs(st, posts));
+                    } else {
+                      assert st' in m'.ToEqs(st, posts)[i];
+                      assert st' in m'.SeqMerge(m'').ToEqs(st, posts)[i] by {
+                        if i in m'.Keys {
+                          assert i in m'.SeqMerge(m'').Keys by {
+                            m'.SeqMergeKeys(m'');
+                          }
+                          forall j: Idx | j < |st| && !(j in m'.SeqMerge(m'').Get(i))
+                            ensures st[j] == st'[j]
+                          {
+                            assert j !in m'.Get(i) by {
+                              if j in m'.Get(i) {
+                                m'.SeqMergeGet1'(m'', j, i);
+                              }
+                            }
+                          }
+                        }
+                      }
+                    }
+                  }
+                }
+              }
+            }
+          }
+      }
+      }
+    } else {
 
-  // // function SeqProcess(ss: seq<Stmt>): (set<Idx>, bool) 
-  // //   ensures forall v <- SeqProcess(ss).0 :: v < SeqDepth(ss)
-  // //   decreases ss
-  // // {
-  // //   if ss == [] then ({}, true) else
-  // //     var (v0, b0) := Process(ss[0]);
-  // //     if b0 then
-  // //       var (v1, b1) := SeqProcess(ss[1..]);
-  // //       (v0 + v1, b0 || b1)
-  // //     else
-  // //       (v0, b0)
-  // // }
+    }
 
-  // function PairToSet(p: (set<Idx>, bool)): set<Idx> {
-  //   if p.1 then p.0 else {}
-  // }
+  }
 
-  // ghost function EqsTo(vars: set<Idx>, st: State): iset<State> 
-  //   requires forall v <- vars :: v < |st|
-  // {
-  //   iset st': State | 
-  //     && |st'| == |st|
-  //     && forall i: Idx :: i < |st| && i !in vars ==> st'[i] == st[i]
-  // }
+  function Process(stmt: Stmt): set<Idx> 
+    ensures forall v <- Process(stmt) :: v < stmt.Depth()
+  {
+    var vs := Process'(stmt);
+    if 0 in vs.Keys then vs[0] else {}
+  } 
+
+  function PairToSet(p: (set<Idx>, bool)): set<Idx> {
+    if p.1 then p.0 else {}
+  }
+
+  ghost function EqsTo(vars: set<Idx>, st: State): iset<State> 
+    requires forall v <- vars :: v < |st|
+  {
+    iset st': State | 
+      && |st'| == |st|
+      && forall i: Idx :: i < |st| && i !in vars ==> st'[i] == st[i]
+  }
 
 
-  // lemma Correct'(stmt: Stmt, st: State, vars: set<Idx>, posts: Omni.Continuation, b : bool) 
-  //   requires forall v <- vars :: v < |st|
-  //   requires Omni.Sem(stmt, st, posts)
-  //   requires Process(stmt) == vars
-  //   ensures Omni.Sem(stmt, st, posts.UpdateHead(posts.head * EqsTo(vars, st)))
+  lemma Correct'(stmt: Stmt, st: State, vars: set<Idx>, posts: Omni.Continuation) 
+    requires forall v <- vars :: v < |st|
+    requires Omni.Sem(stmt, st, posts)
+    requires Process(stmt) == vars
+    ensures Omni.Sem(stmt, st, posts.UpdateHead(posts.head * EqsTo(vars, st)))
+  {
+    Process'Correct(stmt, st, Process'(stmt), posts);
+    Omni.SemCons(stmt, st, Process'(stmt).ToEqs(st, posts), posts.UpdateHead(posts.head * EqsTo(vars, st)));
+  }
 
-  // lemma Correct(stmt: Stmt, st: State, st': State, vars: set<Idx>, posts: Omni.Continuation, post: iset<State>) 
-  //   requires forall v <- vars :: v < |st'|
-  //   requires Omni.Sem(stmt, st, posts.UpdateHead(post))
-  //   requires Process(stmt) == vars
-  //   requires st in EqsTo(vars, st')
-  //   ensures Omni.Sem(stmt, st, posts.UpdateHead(post * EqsTo(vars, st')))
-    
-// }
+  lemma Correct(stmt: Stmt, st: State, st': State, vars: set<Idx>, posts: Omni.Continuation, post: iset<State>) 
+    requires forall v <- vars :: v < |st'|
+    requires Omni.Sem(stmt, st, posts.UpdateHead(post))
+    requires Process(stmt) == vars
+    requires st in EqsTo(vars, st')
+    ensures Omni.Sem(stmt, st, posts.UpdateHead(post * EqsTo(vars, st')))
+  {
+    Correct'(stmt, st, vars, posts.UpdateHead(post));
+    assert posts.UpdateHead(post).UpdateHead(posts.UpdateHead(post).head * EqsTo(vars, st)) == posts.UpdateHead(post * EqsTo(vars, st));
+    Omni.SemCons(stmt, st, posts.UpdateHead(post * EqsTo(vars, st)), posts.UpdateHead(post * EqsTo(vars, st')));
+  }
+}
